lib/Lib.Sequence.Lemmas.fsti
@@ -36,7 +36,7 @@ val slice_index: #a:Type -> #len:size_nat -> s:lseq a len -> start:size_nat -> f
 
 val update_sub_index: #a:Type -> #len:size_nat -> s:lseq a len -> start:size_nat -> n:size_nat{start + n <= len} -> x:lseq a n -> i:size_nat{i < n} -> Lemma
 		  (requires True)
-		  (ensures (index (update_sub s start n x) i == 
+		  (ensures (index (update_sub s start n x) i ==
 			    (if i < start then index s i else
 			     if i >= start + n then index s i else
 			     index x (i - start))))
@@ -44,21 +44,22 @@ val update_sub_index: #a:Type -> #len:size_nat -> s:lseq a len -> start:size_nat
 
 val update_slice_index: #a:Type -> #len:size_nat -> s:lseq a len -> start:size_nat -> fin:size_nat{start <= fin /\ fin <= len} -> x:lseq a (fin - start) -> i:size_nat{i < fin - start} -> Lemma
 		  (requires True)
-		  (ensures (index (update_slice s start fin x) i == 
+		  (ensures (index (update_slice s start fin x) i ==
 			    (if i < start then index s i else
 			     if i >= fin then index s i else
 			     index x (i - start))))
 		  [SMTPat (index (update_slice s start fin x) i )]
 
-val map_index: #a:Type -> #b:Type -> #len:size_nat -> f:(a -> Tot b) -> s:lseq a len -> i:size_nat{i < len} -> Lemma 
+val map_index: #a:Type -> #b:Type -> #len:size_nat -> f:(a -> Tot b) -> s:lseq a len -> i:size_nat{i < len} -> Lemma
 		  (requires True)
 		  (ensures (index (map f s) i == f (index s i)))
 		  [SMTPat (index (map f s) i)]
 
-val map2_index: #a:Type -> #b:Type -> #c:Type -> #len:size_nat -> f:(a -> b ->  Tot c) -> s1:lseq a len -> s2:lseq b len -> i:size_nat{i < len} -> Lemma 
+val map2_index: #a:Type -> #b:Type -> #c:Type -> #len:size_nat -> f:(a -> b ->  Tot c) -> s1:lseq a len -> s2:lseq b len -> i:size_nat{i < len} -> Lemma
 		  (requires True)
 		  (ensures (index (map2 f s1 s2) i == f (index s1 i) (index s2 i)))
 		  [SMTPat (index (map2 f s1 s2) i)]
-
-
-
+//FStar.Seq.Properties.append_slices
+val concat_subs:
+  #a:Type -> #len1:size_nat -> #len2:size_nat{len1 + len2 <= maxint SIZE} -> s1:lseq a len1 -> s2:lseq a len2 -> Lemma
+  (equal s1 (sub (concat s1 s2) 0 len1) /\ equal s2 (sub (concat s1 s2) len1 len2))
