lib/fst/Lib.ByteSequence.fst
@@ -6,6 +6,7 @@ open Lib.Sequence
 open Lib.RawIntTypes
 
 let to_lbytes (s:bytes) = s
+
 let to_bytes #len (s:lbytes len) = s
 
 private
@@ -15,10 +16,10 @@ val nat_from_intseq_be_:#t:m_inttype -> #len:size_nat -> b:intseq t len -> Tot (
 let rec nat_from_intseq_be_ #t #len b =
   if len = 0 then 0
   else
-    let l = uint_to_nat #t (last #(uint_t t) #len b) in
-    let pre : intseq t (decr len) = prefix #(uint_t t) #len b (decr len) in
+    let l = uint_to_nat #t (index b (len - 1)) in
+    let pre : intseq t (decr len) = sub b 0 (decr len) in //prefix #(uint_t t) #len b (decr len)
     let shift = pow2 (bits t) in
-    let n' : n:nat{n < pow2 ((len-1) * bits t)}  = nat_from_intseq_be_ #t #(decr len) pre in
+    let n': n:nat{n < pow2 ((len-1) * bits t)} = nat_from_intseq_be_ #t #(decr len) pre in
     assert (l <= shift - 1);
     assert (l + shift * n' <= shift * (n' + 1) - 1);
     assert (n' + 1 <= pow2 ((len -1) * bits t));
@@ -30,15 +31,14 @@ let rec nat_from_intseq_be_ #t #len b =
 
 let nat_from_intseq_be = nat_from_intseq_be_
 
-
 val nat_from_intseq_le_:#t:m_inttype -> #len:size_nat -> b:intseq t len -> Tot (n:nat{n < pow2 (len * bits t)}) (decreases (len))
 let rec nat_from_intseq_le_ #t #len (b:intseq t len)  =
-  match len,b with
-  | 0, _ -> (0)
-  | _, h::tt ->
+  if len = 0 then 0
+  else
     let shift = pow2 (bits t) in
-    let n' : n:nat{n < pow2 ((len-1) * bits t)}  = nat_from_intseq_le_ #t #(decr len) tt in
-    let l = uint_to_nat #t h in
+    let tt:intseq t (decr len) = sub b 1 (decr len) in
+    let n' : n:nat{n < pow2 ((len-1) * bits t)} = nat_from_intseq_le_ #t #(decr len) tt in
+    let l = uint_to_nat #t (index b 0) in
     assert (l <= shift - 1);
     assert (l + shift * n' <= shift * (n' + 1) - 1);
     assert (n' + 1 <= pow2 ((len -1) * bits t));
@@ -55,25 +55,31 @@ val nat_to_bytes_be_:
   len:size_nat -> n:nat{ n < pow2 (8 * len)} ->
   Tot (b:intseq U8 len {n == nat_from_intseq_be #U8 #len b}) (decreases (len))
 let rec nat_to_bytes_be_ len n =
-  if len = 0 then []
+  if len = 0 then create #(uint_t U8) len (nat_to_uint 0)
   else (
     let len' = decr len in
     let byte = u8 (n % 256) in
-    let n' =  n / 256 in
+    let n' = n / 256 in
     Math.Lemmas.pow2_plus 8 (8 * len');
-    assert( n' < pow2 (8 * len' ));
+    assert (n' < pow2 (8 * len'));
     let b' : intseq U8 len' = nat_to_bytes_be_ len' n' in
-    let b  : intseq U8 len = snoc #uint8 #len' b' byte in
-    assert(b' == prefix b len');
-    assert(byte == last #uint8 #len b);
+    //let b  : intseq U8 len = snoc #uint8 #len' b' byte in
+    let b  : intseq U8 len = concat b' (create 1 byte) in
+    Lib.Sequence.Lemmas.concat_subs b' (create 1 byte);
+    assert (index (create 1 byte) 0 == byte);
+    assert (b' == sub b 0 len');
+    assert (create 1 byte == sub b (decr len) 1);
+    assert (index (sub b (decr len) 1) 0 == index b (decr len));
+    assert (byte == index b (decr len));
     b)
+
 let nat_to_bytes_be = nat_to_bytes_be_
 
 val nat_to_bytes_le_:
   len:size_nat -> n:nat{n < pow2 (8 * len)} ->
   Tot (b:intseq U8 len {n == nat_from_intseq_le #U8 #len b}) (decreases (len))
 let rec nat_to_bytes_le_ len n =
-  if len = 0 then  []
+  if len = 0 then create #(uint_t U8) len (nat_to_uint 0)
   else
     let len = decr len in
     let byte = u8 (n % 256) in
@@ -81,7 +87,13 @@ let rec nat_to_bytes_le_ len n =
     Math.Lemmas.pow2_plus 8 (8 * len);
     assert(n' < pow2 (8 * len ));
     let b' : intseq U8 len = nat_to_bytes_le_ len n' in
-    let b = byte :: b' in
+    let b = concat (create 1 byte) b' in
+    Lib.Sequence.Lemmas.concat_subs (create 1 byte) b';
+    assert (index (create 1 byte) 0 == byte);
+    assert (b' == sub b 1 len);
+    assert (create 1 byte == sub b 0 1);
+    assert (index (sub b 0 1) 0 == index b 0);
+    assert (byte == index b 0);
     b
 
 let nat_to_bytes_le = nat_to_bytes_le_
@@ -115,4 +127,3 @@ let uints_from_bytes_le #t (#len:size_nat{len * numbytes t < pow2 32}) (b:lbytes
 let uints_from_bytes_be #t (#len:size_nat{len * numbytes t < pow2 32}) (b:lbytes (len * numbytes t)) : intseq t len =
   let l = create #(uint_t t) len (nat_to_uint 0) in
   repeati len (fun i l -> l.[i] <- uint_from_bytes_be (sub b (i * numbytes t) (numbytes t))) l
-
